FormalUrchin/proofs/mirlight_proofs.lean
@@ -90,12 +90,14 @@ theorem getPlaceAddr_returns_some_iff_in_env
     {base : Word} {rest: List Word}
     (env: Env) (place: Place) (addr: Addr) (offset: Word) (anyty: TyVal) (anytag: mir.Tag) :
     place = base :: rest →
-    getPlaceOffset (base :: rest) anyty = some offset →
+    getPlaceOffset place anyty = some offset →
     env.find? base = some (addr, anyty, anytag) →
     getPlaceAddr place env = some (addr + offset) := by
-  intros h_src h_ty_validty h_InEnv
-  simp [getPlaceAddr, h_src, h_InEnv, h_ty_validty]
+  intros h_src h_getPlaceOffset h_InEnv
+  simp [h_src] at h_getPlaceOffset
+  simp [getPlaceAddr, h_src, h_InEnv, h_getPlaceOffset]
 
+@[simp]
 theorem copyFromMem_returns_value
     (ap: accessperm.AccessPerms)
      (src_baseaddr: Addr) (offset: Word) (values : List MemValue)
@@ -110,7 +112,7 @@ theorem copyFromMem_returns_value
     -- mir step
     env.find? srcbase = some (src_baseaddr, srcty, srctag) →
     mir.getPlaceType src env = some srcty →
-    getPlaceOffset (srcbase :: srcrest) srcty = some offset →
+    getPlaceOffset src srcty = some offset →
     mir.typeSize srcty = values.length →
     RExprToValFn (mir.RExpr.CopyOp src) env mem ap = RhsResult.Ok values srcty ap mem := by
   intros h_src h_val h_memhasvalues h_srcInEnv h_getPlaceTy h_getPlaceOffset h_tysz
@@ -118,3 +120,295 @@ theorem copyFromMem_returns_value
     readWordSeq_returns_sequence_of_bytes mem (src_baseaddr + offset) values h_memhasvalues
   have h_getPlaceAddr := getPlaceAddr_returns_some_iff_in_env env src src_baseaddr offset srcty srctag h_src h_getPlaceOffset h_srcInEnv
   simp [RExprToValFn, h_getPlaceAddr, h_srcInEnv, h_getPlaceTy, h_read_word_seq, h_tysz, h_val]
+
+
+theorem findval_after_insert (mem : Mem) (addr : Word) (head : MemValue) :
+  -- The `insert` function ensures that `find?` will return the newly inserted value for the given key.
+  Lean.AssocList.find? addr (Lean.AssocList.insert mem.mMap addr head) = some head := by
+  simp [Lean.AssocList.insert]
+  by_cases h_contains : Lean.AssocList.contains addr mem.mMap
+  case pos =>
+    simp [Lean.AssocList.find?, Lean.AssocList.replace, h_contains]
+    
+  case neg =>
+    simp [Lean.AssocList.find?, Lean.AssocList.cons, h_contains]
+
+theorem find_after_insert (mem : Mem) (addr : Word) (head : MemValue) (tail : List MemValue) :
+  -- The `insert` function ensures that `find?` will return the newly inserted value for the given key.
+  Lean.AssocList.find? addr (Lean.AssocList.insert (WriteWordSeq mem (addr + 1) tail).mMap addr head) = some head := by
+  simp [Lean.AssocList.find?, Lean.AssocList.insert]
+
+theorem insert_only_updates_key (m : Lean.AssocList Word MemValue) (location : Word) (val : MemValue) (k : Word) :
+  ¬location = k →
+  Lean.AssocList.find? k (Lean.AssocList.insert m location val) = Lean.AssocList.find? k m := by
+  intros h_cond
+  simp [Lean.AssocList.insert, Lean.AssocList.find?]
+  -- Use `h_cond` to deduce `location == k = false`
+  sorry
+
+theorem writeWordSeq_returns_word (mem : Mem) (mem': Mem) (addr : Word) (addr': Word) (value : MemValue) :
+  WriteWordSeq mem addr [value] = mem' →
+  (if addr' = addr then
+    mem'.mMap.find? addr' = some (value)
+  else
+    mem'.mMap.find? addr' = mem.mMap.find? addr') := by
+
+  intros h_writewordseq
+  by_cases h_addr_eq: addr' = addr
+  case pos =>
+    simp [h_addr_eq]
+    simp [WriteWordSeq] at h_writewordseq
+    simp [←h_writewordseq]
+    have h_find_after_insert := findval_after_insert mem addr value
+    rw [←h_addr_eq]
+    rw [←h_addr_eq] at h_find_after_insert
+    exact h_find_after_insert
+  case neg =>
+    simp [h_addr_eq, ←h_writewordseq]
+    simp [Eq.comm] at h_addr_eq
+    have h_nomemchange := insert_only_updates_key mem.mMap addr value addr' h_addr_eq
+    exact h_nomemchange
+
+theorem sub_lt_of_lt_add {a b c : Nat} : (c > 0) → (a < c + b) → a - b < c := by
+  intros hpos hlt
+  cases Nat.lt_or_ge a b with
+  | inl hlt =>
+    rw [Nat.sub_eq_zero_of_le (Nat.le_of_lt hlt)]
+    exact hpos
+  | inr hge =>
+    have h1 : a - b + b < c + b := by
+      rw [Nat.sub_add_cancel hge]
+      exact hlt
+    apply Nat.lt_of_add_lt_add_right h1
+
+theorem WriteWordSeq_concat {mem'': Mem} (mem : Mem) (addr : Word) (head : MemValue) (tail : List MemValue) :
+  ∃ mem' : Mem, (WriteWordSeq mem (addr + 1) tail = mem' ∧
+   WriteWordSeq mem' addr [head] = mem'') ↔
+  WriteWordSeq mem addr (head :: tail) = mem'' := by
+  let mem' := WriteWordSeq mem (addr + 1) tail
+  exists mem'
+  apply Iff.intro
+  {
+    intro h
+    obtain ⟨h_tail, h_head⟩ := h
+    simp [WriteWordSeq]
+    simp [WriteWordSeq] at h_head
+    rw [← h_tail] at h_head
+    exact h_head
+  }
+  {
+    intro h
+    simp [WriteWordSeq]
+    simp [WriteWordSeq] at h
+
+    apply And.intro
+    {
+      rfl
+    }
+    {
+      simp [mem']
+      exact h
+    }
+  }
+
+theorem h_succ_is_plus1 {a b : Nat} (h : a < b) : a + 1 < b + 1 := by
+  exact Nat.succ_lt_succ h
+
+theorem get_tail_eq
+  {α : Type}
+  {addr addr' : Nat}
+  (head : α) (tail : List α)
+  (h₁ : addr' - addr < tail.length + 1)
+  (h₂ : addr' ≥ addr + 1)
+  (h_tail : tail.length > 0) :
+  (head :: tail).get ⟨addr' - addr, h₁⟩ = tail[addr' - (addr + 1)] := by
+  -- let n := addr' - addr
+  let n := addr' - addr
+  have hn_pos : n ≥ 1 := by
+    have hn_pos : addr' - addr ≥ 1 := by
+      apply Nat.le_sub_of_add_le
+      rw [Nat.add_comm] at h₂
+      exact h₂
+    exact hn_pos
+
+  let m := addr' - (addr + 1)
+  have h_m_eq : n = m + 1 := by
+    have h_eq' : addr' - (addr + 1) = addr' - addr  - 1 := by
+      rw [Nat.sub_sub]
+    symm
+    simp [h_eq', m, n]
+    have h_addr_ge : 1 ≤ addr' - addr := by
+      apply Nat.le_sub_of_add_le
+      rw [Nat.add_comm] at h₂
+      exact h₂
+    apply Nat.sub_add_cancel h_addr_ge
+    -- Prove bounds for indexing
+  have h_n_lt : n < (head :: tail).length := by
+    change (addr' - addr) < (head :: tail).length
+    simp
+    exact h₁
+  have h_eq' : addr' - (addr + 1) = addr' - addr  - 1 := by
+        rw [Nat.sub_sub]
+  have h_m_lt : m < tail.length := by
+    change addr' - (addr + 1) < tail.length
+    let hh_1 := sub_lt_of_lt_add h_tail h₁
+    rw [←h_eq'] at hh_1
+    exact hh_1
+  change (head :: tail).get ⟨n, h_n_lt⟩ = tail[m]
+  simp [h_m_eq]
+
+
+theorem writeWordSeq_returns_sequence_of_words  {mem': Mem} (mem : Mem) (addr : Word) (addr': Word) (values : List MemValue) :
+  ∃ mem' : Mem, WriteWordSeq mem addr values = mem' →
+  (if h : addr' ≥ addr ∧ addr' - addr  < values.length then
+    mem'.mMap.find? addr' = some (values.get ⟨addr' - addr, h.right⟩)
+  else
+    mem'.mMap.find? addr' = mem.mMap.find? addr') := by
+  exists mem'
+  intros h_write
+  induction values generalizing mem' addr
+  case nil =>
+    simp [WriteWordSeq] at h_write
+    have h_mem : mem' = mem := by
+      rw [←h_write]
+    subst h_mem
+    simp
+  case cons head tail ih =>
+    obtain ⟨mem_intmd, h_iff⟩ := WriteWordSeq_concat mem addr head tail
+    --specialize ih (addr + 1)
+    let h_0 := (h_iff.mpr h_write).left
+    let ih_1 := ih (addr + 1) h_0
+    let h_1 := (h_iff.mpr h_write).right
+    let h_2 := writeWordSeq_returns_word mem_intmd mem' addr addr' head
+    let h_3 := h_2 h_1
+    simp at ih_1
+    simp
+    let h_4 := And.intro h_3 ih_1
+    simp at h_4
+    by_cases h_cond : addr' ≥ addr ∧ addr' - addr < tail.length + 1
+    case pos =>
+      simp [h_cond]
+      by_cases h_addr : addr' = addr
+      case pos =>
+        simp [h_addr] at h_3
+        simp [h_addr]
+        exact h_3
+      case neg =>
+        have h_addr_tail :
+          addr' ≥ addr + 1 := by
+          let h_addr_in_tail := And.intro h_addr h_cond.left
+          -- Extract the two parts of the hypothesis
+          obtain ⟨h_neq, h_ge⟩ := h_addr_in_tail
+          -- Convert `addr' ≥ addr` and `addr' ≠ addr` to `addr' > addr`
+          have h_gt : addr' > addr := Nat.lt_of_le_of_ne h_ge (Ne.symm h_neq)
+          -- Apply the fact that `addr' > addr` implies `addr + 1 ≤ addr'`
+          exact Nat.succ_le_of_lt h_gt
+        by_cases h_no_tail : tail = []
+        case pos =>
+          -- This is an impossible case
+          -- TODO: simplify the proof
+          have h_tail_zero_length : tail.length = 0 := by
+            rw [h_no_tail]
+            simp
+          simp [h_tail_zero_length, h_addr_tail] at h_cond
+          let h_cond_right :=  Nat.le_of_sub_eq_zero h_cond.right
+          let h_cond' :=  Nat.le_antisymm h_cond.left h_cond_right
+          have h_contradiction : False := by
+            rw [h_cond'] at h_addr
+            exact h_addr rfl
+          contradiction
+        case neg =>
+          have h_tail_ne_zero_length : tail.length > 0 := by
+            cases tail with
+            | nil => contradiction
+            | cons _ _ => simp [List.length]
+          let h_1_rgt_to_lft := sub_lt_of_lt_add h_tail_ne_zero_length h_cond.right
+          have h_1_rgt_to_lft_rw : addr' - (addr + 1) < tail.length := by
+            rw [Nat.sub_add_eq]
+            exact h_1_rgt_to_lft
+          simp [h_cond, h_addr_tail, h_1_rgt_to_lft_rw] at ih_1
+          have h_addr_ne :
+            addr' ≠ addr := by
+            exact Ne.symm (Ne.symm h_addr)
+          simp [h_addr_ne] at h_2
+          let h_22 := h_2 h_1
+          rw [h_22, ih_1]
+          let h_skip_head := get_tail_eq head tail h_cond.right h_addr_tail h_tail_ne_zero_length
+          simp [←h_skip_head]
+
+    case neg =>
+      simp [h_cond]
+      have h_ih_neg :
+        (addr + 1 ≤ addr' ∧ addr' - (addr + 1) < tail.length) → addr' ≥ addr ∧ addr' - addr < tail.length + 1 := by
+        intros h_subset
+        obtain ⟨h_ge, h_lt⟩ := h_subset
+        have h_ge' : addr' ≥ addr := by
+          exact Nat.le_of_succ_le h_ge
+        have h_eq' : addr' - (addr + 1) = addr' - addr  - 1 := by
+          rw [Nat.sub_sub]
+        have h_lt' : addr' - addr < tail.length + 1 := by
+          let h_eq := h_eq'
+          rw [h_eq'] at h_lt
+          have h_addr_ge : 1 ≤ addr' - addr := by
+            apply Nat.le_sub_of_add_le
+            rw [Nat.add_comm] at h_ge
+            exact h_ge
+          let h_x := Nat.sub_add_cancel h_addr_ge
+          let h_x1 := h_succ_is_plus1 h_lt
+          rw [h_x] at h_x1
+          exact h_x1
+        exact And.intro h_ge' h_lt'
+      let hhhaaa := Not.imp h_cond h_ih_neg
+      simp [hhhaaa] at ih_1
+      have h_ih_neg2 :
+        addr = addr' → addr' ≥ addr ∧ addr' - addr < tail.length + 1 := by
+        intros h_eq
+        rw [h_eq] at h_cond
+        have h_ge : addr' ≥ addr := by
+          exact Nat.le_of_eq h_eq
+        have h_lt : addr' - addr < tail.length + 1 := by
+          rw [Nat.sub_self] at h_cond
+          simp [h_eq]
+        exact And.intro h_ge h_lt
+      let hhaaa2 := (Not.imp h_cond h_ih_neg2)
+      have hhaaa3 :
+        addr' ≠ addr := by
+        exact Ne.symm hhaaa2
+      simp [hhaaa3] at h_3
+      rw [←h_3] at ih_1
+      exact ih_1
+
+@[simp]
+theorem EvalStep_copy
+    (prog: Prog) (bb: BB) (pc: PC) (pc': PC)
+    (ap: accessperm.AccessPerms)
+    (src_baseaddr: Addr) (offset: Word) (values : List MemValue)
+    (dst_baseaddr: Addr) (dst_offset: Word) (values : List MemValue)
+    (env: Env) (env': Env)
+    (srcbase : Word)
+    (srcrest : Place)
+    (src : Place) (srcty: TyVal) (srctag: mir.Tag)
+    (dst : Place) (dsttag: mir.Tag)
+    (mem: Mem) (mem': Mem) :
+    --  pre condition
+    (h_src : src = srcbase :: srcrest) →
+    (h_dst : dst = dstbase :: dstrest) →
+    (h_val : values ≠ []) →
+    (∀ i, (h: i < values.length) → mem.mMap.find? (src_baseaddr + offset + i) = some (values.get ⟨i, h⟩)) →
+    env.find? srcbase = some (src_baseaddr, srcty, srctag) →
+    mir.getPlaceType src env = some srcty →
+    getPlaceOffset src srcty = some offset →
+    mir.typeSize srcty = values.length →
+    -- mir step
+    Eval2 (bb, pc, prog, env, mem, ap) (bb, pc', prog, env', mem', ap) →
+    -- post condition
+    ∀ k', if k' == dstbase then env'.find? k' = some (dst_baseaddr, srcty, dsttag)
+        else env'.find? k' = env.find? k' →
+    getPlaceOffset dst srcty = some dst_offset →
+    (h_addr: dst_addr = dst_baseaddr + dst_offset) →
+    (prog.find? bb = some [mir.Stmt.Assgn dst (mir.RExpr.CopyOp (srcbase :: srcrest))]) →
+    (∀ addr', i = addr' - dst_addr → if h : addr' ≥ dst_addr ∧ i < values.length then
+      mem'.mMap.find? addr' = some (values.get ⟨i, h.right⟩)
+    else
+      mem'.mMap.find? addr' = mem.mMap.find? addr') := by
+  sorry
